Finish proof

src/computability/DFA.lean
@@ -45,9 +45,12 @@ def eval := M.eval_from M.start
 def accepts : language α :=
 λ x, M.eval x ∈ M.accept
 
+lemma mem_accepts (x : list α) : x ∈ M.accepts ↔ M.eval_from M.start x ∈ M.accept := by refl
+
+/-- `M.state_path s x` is the states the DFA passes through when evalulating `M.eval_from s x` -/
 def state_path : σ → list α → list σ
 | start [] := [start]
-| start (a :: x) := M.step start a :: state_path (M.step start a) x
+| start (a :: x) := start :: state_path (M.step start a) x
 
 @[simp] lemma length_state_path (start : σ) (x : list α) :
   (M.state_path start x).length = x.length + 1 :=
@@ -57,23 +60,61 @@ begin
   tauto
 end
 
+lemma nth_le_state_path_eq_eval_from_take (start : σ) (x : list α) (n : ℕ)
+(h : n < (M.state_path start x).length) :
+  (M.state_path start x).nth_le n h = M.eval_from start (x.take n) :=
+begin
+  induction n with n ih generalizing start x,
+  { rw [list.take_zero, eval_from, list.foldl],
+    cases x,
+    all_goals
+    { unfold state_path,
+      rw list.nth_le } },
+  { cases x,
+    { rw [state_path, list.length_singleton, nat.lt_succ_iff, le_zero_iff_eq] at h,
+      contradiction },
+    unfold state_path,
+    rw [list.take, list.nth_le, eval_from, list.foldl],
+    apply ih }
+end
+
+lemma eval_from_of_append (start : σ) (x y : list α) :
+  M.eval_from start (x ++ y) = M.eval_from (M.eval_from start x) y :=
+begin
+  induction x with a x ih generalizing start,
+  { repeat {rw eval_from},
+    rw [list.nil_append, list.foldl] },
+  { rw [list.cons_append, eval_from, list.foldl],
+    apply ih }
+end
+
 variable [fintype σ]
 
 lemma pumping_lemma : ∃ p : ℕ, ∀ x ∈ M.accepts, p ≤ list.length x → ∃ a b c, x = a ++ b ++ c ∧
-  b ≠ [] ∧ (a ++ b).length ≤ p ∧ {a} + language.star {b} + {c} ≤ M.accepts :=
+  b ≠ [] ∧ (a ++ b).length ≤ p ∧ {a} * language.star {b} * {c} ≤ M.accepts :=
 begin
   -- Let p be one more than the number of states in our DFA
   use fintype.card σ + 1,
-  intros x hMx hlen,
+  intros x hx hlen,
 
   -- By pidgeon hole principal the DFA passes though the same state twice in the first p+1 states we
   -- pass through. Let these be the `n`th and `m`th states with `n < m`
-  let state_map : fin (fintype.card σ + 1) → σ := λ n, (M.state_path M.start x).nth_le n begin cases n with n h, rw [length_state_path, fin.coe_mk], apply lt_of_lt_of_le, assumption, omega end,
-  have h := fintype.exists_ne_map_eq_of_card_lt state_map (by norm_num),
+  have hnfintype : ∀ n : fin (fintype.card σ + 1), ↑n < (M.state_path M.start x).length,
+  { intro n,
+    cases n with n h,
+    rw [length_state_path, fin.coe_mk],
+    apply lt_of_lt_of_le h,
+    rw nat.le_add_one_iff,
+    left,
+    assumption },
+  have h := fintype.exists_ne_map_eq_of_card_lt
+    (λ n : fin (fintype.card σ + 1), (M.state_path M.start x).nth_le n (hnfintype n)) (by norm_num),
   rcases h with ⟨ n, m, hneq, heq ⟩,
   cases m with m hm, cases n with n hn,
   wlog hle : n ≤ m using [n m, m n],
   { exact le_total n m },
+  change list.nth_le _ n _ = list.nth_le _ m _ at heq,
+  rw [nth_le_state_path_eq_eval_from_take, nth_le_state_path_eq_eval_from_take] at heq,
 
   -- Now let `a` be the first `n` characters of `x`, `b` be the next `m-n` characters and `c` the
   -- rest
@@ -98,8 +139,38 @@ begin
     left,
     apply le_of_lt,
     assumption },
-  { intro k,
-    -- We now show `a ++ n*b` }
+
+  -- We now show `M` accepts `y := a ++ i*b ++ c` by induction on `i` and showing `a ++ i*b`
+  -- always finishes on the same state
+  rw [language.star_eq_supr_pow, language.mul_supr, language.supr_mul],
+  intros y hy,
+  rw set.mem_Union at hy,
+  cases hy with i hy,
+  rw language.mem_mul at hy,
+  rcases hy with ⟨ a, c, ha, hc, hy ⟩,
+  have hnstate_path : n < (M.state_path M.start x).length,
+  { rw length_state_path,
+    apply lt_of_lt_of_le hn,
+    rw nat.le_add_one_iff,
+    left,
+    assumption },
+  have h : M.eval_from M.start a = (M.state_path M.start x).nth_le n hnstate_path,
+  { induction i with i ih generalizing a y,
+    { rw [pow_zero, mul_one, set.mem_singleton_iff] at ha,
+      rw [ha, list.take_take, min_eq_left hle, ←nth_le_state_path_eq_eval_from_take] },
+    { rw [pow_succ', ←mul_assoc, language.mem_mul] at ha,
+      rcases ha with ⟨ a', b, ha', hb, ha ⟩,
+      specialize ih a' ha' rfl,
+      rw set.mem_singleton_iff at hb,
+      rw [←ha, eval_from_of_append, ih, nth_le_state_path_eq_eval_from_take, hb,
+          ←eval_from_of_append, ←min_eq_left hle, ←list.take_take, min_eq_left hle,
+          list.take_append_drop, list.take_take, min_eq_left hle],
+      exact heq.symm } },
+
+  rw set.mem_singleton_iff at hc,
+  rw [←hy, mem_accepts, eval_from_of_append, h, nth_le_state_path_eq_eval_from_take, heq,
+    ←eval_from_of_append, hc, list.take_append_drop],
+  exact hx
 end
 
 end DFA
